# (PART) Symbolic Derivatives {-}

# Rules of Differentiation



## Derivatives of Familiar Functions

### Constant Rule

The derivative of a constant is 0.
$$\frac{d}{dx}(c)= 0$$

### Linear Function Rule
If $f(x)=mx+b$, then the derivative is the slope $m$.
$$\frac{d}{dx}(mx+b)= m$$

### Power Rule

$$\frac{d}{dx}(x^n)=n x^{n-1}$$

### Trig Rules

$$\frac{d}{dx}\sin(x)=\cos(x)$$
and
$$\frac{d}{dx}\cos(x)=-\sin(x)$$

### Exponential Rules

$$\frac{d}{dx}(e^x)=e^x$$ 
and for any positive number $a >0$, 
$$\frac{d}{dx}(a^x)=(\ln a)a^x$$


### Logarithmic Rules

$$\frac{d}{dx}(\ln (x))=\frac{1}{x}$$
and for any positive number $a >0$, 
$$\frac{d}{dx}(\log_a x)= \frac{1}{\ln (a)} \cdot \frac{1}{x}$$

## Arithmetic Rules for Derivatives

### Constant Multiple Rule

If $c$ is a constant, then
$$\frac{d}{dx}(cf(x))=c\frac{d}{dx}f(x)=cf'(x)$$

### Sum and Difference Rules  

$$\frac{d}{dx}(f(x)+g(x))=\frac{d}{dx}f(x)+\frac{d}{dx}g(x)=f'(x)+g'(x)$$
and
$$\frac{d}{dx}(f(x)-g(x))=\frac{d}{dx}f(x)-\frac{d}{dx}g(x)=f'(x)-g'(x)$$

## Rules for Combinations of Functions

### Product Rule

If $f(x)$ and $g(x)$ are functions then
$$(fg)'=f'g+fg' \phantom{hihi} \text{ or } \phantom{hihi}(1st \cdot 2nd )'=D1st \cdot 2nd + 1st \cdot D2nd$$

### Quotient Rule

If $f(x)$ and $g(x)$ are functions then
$$\left(\frac{f}{g} \right ) '=\frac{gf'-fg'}{g^2} \phantom{hihi}\text{ or } \phantom{hihi}\left(\frac{hi}{lo} \right ) '=\frac{loDhi-hiDlo}{lo^2}$$

### Chain Rule 

If $y=f(t)$ and $t=g(x)$ are functions, then the derivative of $y=f(g(x))$ is given by
$$\frac{dy}{dx}=\frac{dy}{dt}\frac{dt}{dx} \phantom{hihi}\text{ or } \phantom{hihi}\frac{d}{dx}(f(g(x)))=f'(g(x))g'(x)=D(outside)D(inside)$$
 


