# 2.B Dimensional Analysis


## Performing a Dimensional Analysis

Given independent variables $x,y,z$ and dependent variable $w$:

1. Write down the hypothesized "generalized product" $w = k x^a y^b z^c$
2. Write \& simplify the dimensional version $[w] = [x]^a [y]^b [z]^c$
3. List the dimensions of all quantities
4. Invoke dimensional compatibility to solve.
5. Rewrite your equation, marvel at your awesomeness!


## Activities

### Vocal Chord Frequency

The frequency $f$ of the sound of an organism's vocal chords depend on their length $\ell$, tension $s$ (a force) and mass density $\mu$ (mass per unit length). Find a formula for the frequency $f = f(\ell, s, \mu).$

### Mixer Power

A mixer with power $P$ turns a mixer with wings of length $D$ through a liquid of viscosity $H$. Find a formula for the angular velocity $A = A(P,D,H)$. Note that since angles are dimensionless, we have $[A] = 1/T$. The dimensions of viscosity are $[H] = M/(LT)$.

### Velocity of an Ocean Wave

The velocity $V$ of a large ocean wave depends upon the period $P$, the acceleration of gravity $g$, and the density $\mu$ of the water. Find a formula for the velocity $V=V(P,g,\mu)$.



## Solutions

1. We have
$$
\begin{array}{rcl}
f &=& k \ell^a s^b \mu^c \\
[f] &=&  [\ell]^a [s]^b [\mu]^c \\
T^{-1} &=& \left( L\right)^a \left(MLT^{-2}\right)^b \left( M L^{-1}  \right)^c \\
M^0L^0T^{-1} &=& M^{b+c} L^{a+b-c} T^{-2b}
\end{array}
$$
and so we have
$$
0 = b+c \qquad 0 = a+b-c \qquad -1=-2b.
$$
Therefore $b=1/2$ and $c=-1/2$ and $a=-1$. Our formula is
$$
f = k \ell^{-1} s^{1/2} \mu^{-1/2} k \frac{1}{\ell} \sqrt{\frac{s}{\mu}}.
$$
2. We have
$$
\begin{array}{rcl}
A &=& k P^a D^b H^c \\
[A] &=&  [P]^a [D]^b [H]^c \\
T^{-1} &=& \left( ML^2T^{-3}\right)^a L^b \left( M L^{-1} T^{-1}  \right)^c \\
M^0L^0T^{-1} &=& M^{a+c} L^{2a+b-c} T^{-3a-c}
\end{array}
$$
and so  we have
$$
0 = a+c \qquad 0 = 2a+b-c \qquad -1 = -3a-c
$$
which means that $a=1/2$ and $c=-1/2$ and $b=-3/2$. So our final equation is
$$
A = k a^{1/2} b^{-3/2} c^{-1/2} = k \sqrt{\frac{P}{D^3H}}
$$

3. We have
$$
\begin{array}{rcl}
V &=& k P^a g^b \mu^c \\
[V] &=& [P]^a [g]^b [\mu]^c \\
LT^{-1} &=& (T)^a (LT^{-2})^b (ML^{-3})^c \\
 L^1 T^{-1} M^0 &=& L^{b-3c} T^{a-2b} M^{c}
\end{array}
$$
so we have the equations
$$
1 = b - 3c \qquad -1 = a-2b \qquad 0 = c
$$
which means that $c=0$ and $b=1$ and $a=1$. So our final equation is
$$
V = k Pg
$$
